More progress in reorganization.

PropositionalLogic/DeepEmbeddedInstance/KripkeSemantics.v
@@ -6,9 +6,8 @@ Require Import Logic.GeneralLogic.Base.
 Require Import Logic.MinimunLogic.Syntax.
 Require Import Logic.PropositionalLogic.Syntax.
 Require Import Logic.PropositionalLogic.Semantics.Kripke.
+Require Import Logic.PropositionalLogic.KripkeModel.
 Require Import Logic.PropositionalLogic.DeepEmbeddedInstance.PropositionalLanguage.
-
-Module KripkeSemantics.
 
 Import PropositionalLanguage.
 
@@ -22,54 +21,32 @@ Infix "<=" := (Krelation _): TheKripkeSemantics.
 
 Local Open Scope TheKripkeSemantics.
 
-Definition sem (f: frame) := sig (fun s: Ensemble f => forall x y, x <= y -> s x -> s y).
+Definition sem (f: frame) := sig (@upwards_closed_Kdenote f (Krelation f)).
 
-Program Definition sem_and {F: frame} (X: sem F) (Y: sem F): sem F := Semantics.andp X Y.
-Next Obligation.
-  destruct H0.
-  split.
-  + eapply (proj2_sig X); eauto.
-  + eapply (proj2_sig Y); eauto.
-Qed.
-
-Program Definition sem_or {F: frame} (X: sem F) (Y: sem F): sem F :=
-  fun x: F => X x \/ Y x.
-Next Obligation.
-  destruct H0; [left | right].
-  + eapply (proj2_sig X); eauto.
-  + eapply (proj2_sig Y); eauto.
-Qed.
-
-Program Definition sem_imp {F: frame} (X: sem F) (Y: sem F): sem F :=
-  fun x: F =>
-    forall y: F, x <= y -> X y -> Y y.
-Next Obligation.
-  revert H2; apply H0.
-  pose proof @PreOrder_Transitive _ _ (Korder_preorder F).
-  transitivity y; auto.
-Qed.
-
-Program Definition sem_true {F: frame}: sem F :=
-  fun x: F => True.
-
-Program Definition sem_false {F: frame}: sem F :=
-  fun x: F => False.
-
-Definition sem_neg {F: frame} (X: sem F): sem F :=
-  sem_imp X sem_false.
-
-Definition sem_iff {F: frame} (X: sem F) (Y: sem F): sem F :=
-  sem_and (sem_imp X Y) (sem_imp Y X).
-
-Definition denotation {Var: Type} (F: frame) (eval: Var -> sem F): expr Var -> sem F :=
+Program Definition denotation {Var: Type} (F: frame) (eval: Var -> sem F): expr Var -> sem F :=
   fix denotation (x: expr Var): sem F:=
   match x with
-  | andp y z => sem_and (denotation y) (denotation z)
-  | orp y z => sem_or (denotation y) (denotation z)
-  | impp y z => sem_imp (denotation y) (denotation z)
-  | falsep => sem_false
+  | andp y z => @Semantics.andp F (denotation y) (denotation z)
+  | orp y z => @Semantics.orp F (denotation y) (denotation z)
+  | impp y z => @Semantics.impp F (Krelation F) (denotation y) (denotation z)
+  | falsep => @Semantics.falsep F
   | varp p => eval p
   end.
+Next Obligation.
+  apply (@Semantics.andp_closed F (Krelation F) (Krelation_Preorder F));
+  apply (proj2_sig (denotation _)).
+Defined.
+Next Obligation.
+  apply (@Semantics.orp_closed F (Krelation F) (Krelation_Preorder F));
+  apply (proj2_sig (denotation _)).
+Defined.
+Next Obligation.
+  apply (@Semantics.impp_closed F (Krelation F) (Krelation_Preorder F));
+  apply (proj2_sig (denotation _)).
+Defined.
+Next Obligation.
+  apply (@Semantics.falsep_closed F (Krelation F)).
+Defined.
 
 Section KripkeSemantics.
 Context (Var: Type).
@@ -93,22 +70,24 @@ Instance kMD: KripkeModel MD :=
     (fun M => M)
     (fun M m => Build_model M m).
 
+Instance R (M: Kmodel): Relation (Kworlds M) :=
+  @Krelation M.
+
 Instance kiM (M: Kmodel): KripkeIntuitionisticModel (Kworlds M) :=
-  Build_KripkeIntuitionisticModel (Kworlds M) (Korder M) (Korder_preorder _).
+  @Krelation_Preorder M.
 
 Instance SM: Semantics L MD :=
-  Build_Semantics L MD
-   (fun M x => proj1_sig (denotation M (Kvar M) x) (elm M)).
+  Build_Semantics L MD (fun x M => proj1_sig (denotation M (Kvar M) x) (elm M)).
 
 Instance kiSM (M: Kmodel): KripkeIntuitionisticSemantics L MD M SM.
 Proof.
   apply Build_KripkeIntuitionisticSemantics.
   + hnf; simpl; intros.
     eapply (proj2_sig (denotation M (Kvar M) x)); eauto.
-  + split; auto.
-  + split; auto.
-  + split; auto.
-  + intros; simpl. auto.
+  + intros; apply Same_set_refl.
+  + intros; apply Same_set_refl.
+  + intros; apply Same_set_refl.
+  + intros; apply Same_set_refl.
 Defined.
 
 Definition Kmodel_Identity: Kmodel -> Prop := fun M =>
@@ -120,5 +99,4 @@ Definition Kmodel_NoBranch: Kmodel -> Prop := fun M =>
 Definition Kmodel_BranchJoin: Kmodel -> Prop := fun M =>
   BranchJoinKripkeIntuitionisticModel (Kworlds M).
 
-End KripkeSemantics.
 End KripkeSemantics.
